cleanup to avoid extracting crap

coq/Word/WordInterface.v
@@ -4,8 +4,6 @@ Require Import Coq.Logic.ProofIrrelevance.
 Require Import Coq.Structures.Equalities.
 Require Import PArith.BinPos.
 Require Import NArith.BinNat.
-Require Import Bag.TotalOrder.
-
 Local Open Scope N_scope.
 
 Module Type WORD <: MiniDecidableType.
@@ -31,7 +29,20 @@ Module Type WIDTH.
 
 End WIDTH.
 
-Module MakeWord (Width : WIDTH).
+Module Type MAKEWORD.
+
+  Local Open Scope N_scope.
+
+  Parameter width : positive.
+  
+  Inductive Word : Type := 
+  | Mk : forall (v : N), v < 2 ^ N.pos width -> Word.
+
+  Definition t := Word.
+
+End MAKEWORD.
+
+Module MakeWord (Width : WIDTH) <: MAKEWORD.
 
   Local Open Scope N_scope.
 
@@ -44,92 +55,7 @@ Module MakeWord (Width : WIDTH).
 
   Definition zero : t := @Mk 0 eq_refl.
 
-  Lemma eq_dec : forall (m n : t), { m = n } + { m <> n }.
-  Proof.
-    intros.
-    destruct m, n.
-    assert ({v = v0} + {v <> v0}) as J.
-    { apply N.eq_dec. }
-    destruct J; subst.
-    + left.
-      f_equal.
-      apply proof_irrelevance.
-    + right.
-      unfold not.
-      intros.
-      inversion H; subst.
-      contradiction n.
-      reflexivity.
-  Qed.
-
-  Definition le (x y : t) : Prop :=
-    match (x, y) with
-      | (Mk m _, Mk n _) => m <= n
-    end.
-
-  Lemma le_reflexivity : forall (x : t), le x x.
-  Proof with auto.
-    intros.
-    destruct x...
-    apply N.le_refl.
-  Qed.
-
-  Lemma le_antisymmetry : forall (x y : t), le x y -> le y x -> x = y.
-  Proof with eauto.
-    intros.
-    destruct x, y.
-    unfold le in *.
-    apply N.lt_eq_cases in H.
-    apply N.lt_eq_cases in H0.
-    destruct H, H0...
-    + assert (v < v). eapply N.lt_trans...
-      apply N.lt_irrefl in H1. inversion H1.
-    + subst...
-      assert (l = l0). apply proof_irrelevance.
-      subst...
-    + subst...
-      assert (l = l0). apply proof_irrelevance.
-      subst...
-    + clear H0; subst.
-      assert (l = l0). apply proof_irrelevance.
-      subst...
-  Qed.
-
-  Lemma le_transitivity : forall (x y z : t), le x y -> le y z -> le x z.
-  Proof with eauto.
-    intros.
-    destruct x, y, z.
-    unfold le in *.
-    eapply N.le_trans...
-  Qed.
-
-  Lemma le_compare : forall (x y : t), { le x y } + { le y x }.
-  Proof with eauto.
-    intros.
-    destruct x, y.
-    unfold le in *.
-    remember (N.compare v v0) as cmp eqn:J.
-    symmetry in J.
-    destruct cmp.
-    + apply N.compare_eq_iff in J.
-      subst.
-      left...
-      apply N.lt_eq_cases...
-    + rewrite ->  N.compare_lt_iff in J.
-      left.
-      apply N.lt_eq_cases...
-    + rewrite ->  N.compare_gt_iff in J.
-      right.
-      apply N.lt_eq_cases...
-  Qed.
- 
-  Instance TotalOrder :  TotalOrder le := {
-    reflexivity := le_reflexivity;
-    antisymmetry := le_antisymmetry;
-    transitivity := le_transitivity;
-    compare := le_compare;
-    eqdec := eq_dec
-  }.
+  Parameter eq_dec : forall (m n : t), { m = n } + { m <> n }.
 
 End MakeWord.
 
@@ -227,9 +153,6 @@ Module Word64 <: WORD.
 
 End Word64.
 
-Existing Instances Word8.TotalOrder Word16.TotalOrder Word12.TotalOrder
-  Word32.TotalOrder Word48.TotalOrder Word64.TotalOrder.
-
 Extract Constant Word16.pred => "(fun n -> if n = 0 then 0 else n - 1)". (* TODO: really fix this (JNF) *)
 Extract Constant Word16.max_value => "65535".
 
@@ -253,9 +176,3 @@ Extract Constant Word16.zero => "0".
 Extract Constant Word32.zero => "Int32.zero".
 Extract Constant Word48.zero => "Int64.zero".
 Extract Constant Word64.zero => "Int64.zero".
-
-Extract Constant Word8.le_compare => "(<=)".
-Extract Constant Word16.le_compare => "(<=)".
-Extract Constant Word32.le_compare => "(fun x y -> Int32.compare x y <= 0)".
-Extract Constant Word48.le_compare => "(fun x y -> Int64.compare x y <= 0)".
-Extract Constant Word64.le_compare => "(fun x y -> Int64.compare x y <= 0)".
